src/Trace.v
@@ -348,6 +348,7 @@ Module Euf_Checker.
   | SplDistinctElim (pos:int) (orig:clause_id) (res:_lit)
   (* Bit-blasting *)
   | BBVar (pos:int) (res:_lit)
+  | BBConst (pos:int) (res:_lit)
   | BBOp (pos:int) (orig1 orig2:clause_id) (res:_lit)
   | BBAdd (pos:int) (orig1 orig2:clause_id) (res:_lit)
   | BBMul (pos:int) (orig1 orig2:clause_id) (res:_lit)
@@ -382,7 +383,8 @@ Module Euf_Checker.
       | LiaDiseq pos l => S.set_clause s pos (check_diseq t_form t_atom l)
       | SplArith pos orig res l => S.set_clause s pos (check_spl_arith t_form t_atom (S.get s orig) res l)
       | SplDistinctElim pos orig res => S.set_clause s pos (check_distinct_elim t_form t_atom (S.get s orig) res)
-      | BBVar pos res => S.set_clause s pos (check_bbVar (* t_func *) t_atom t_form res)
+      | BBVar pos res => S.set_clause s pos (check_bbVar t_atom t_form res)
+      | BBConst pos res => S.set_clause s pos (check_bbConst t_atom t_form res)
       | BBOp pos orig1 orig2 res => S.set_clause s pos (check_bbOp t_atom t_form s orig1 orig2 res)
       | BBAdd pos orig1 orig2 res => S.set_clause s pos (check_bbAdd t_atom t_form s orig1 orig2 res)
       | BBMul pos orig1 orig2 res => S.set_clause s pos (check_bbMult t_atom t_form s orig1 orig2 res)
@@ -397,7 +399,7 @@ Module Euf_Checker.
       forall s, S.valid rho s ->
         forall st : step, S.valid rho (step_checker s st).
   Proof.
-    intros rho H1 H2 H10 s Hs. destruct (Form.check_form_correct (Atom.interp_form_hatom t_i t_func t_atom) (Atom.interp_form_hatom_bv t_i t_func t_atom) _ H1) as [[Ht1 Ht2] Ht3]. destruct (Atom.check_atom_correct _ H2) as [Ha1 Ha2]. intros [pos res|pos cid c|pos cid lf|pos|pos|pos l|pos l|pos l i|pos cid|pos cid|pos cid i|pos l fl|pos l fl|pos l1 l2 fl|pos cl c|pos l|pos orig res l|pos orig res|pos res|pos orig1 orig2 res|pos orig1 orig2 res|pos orig1 orig2 res|pos orig1 orig2 res|pos prem_id prem concl p]; simpl; try apply S.valid_set_clause; auto.
+    intros rho H1 H2 H10 s Hs. destruct (Form.check_form_correct (Atom.interp_form_hatom t_i t_func t_atom) (Atom.interp_form_hatom_bv t_i t_func t_atom) _ H1) as [[Ht1 Ht2] Ht3]. destruct (Atom.check_atom_correct _ H2) as [Ha1 Ha2]. intros [pos res|pos cid c|pos cid lf|pos|pos|pos l|pos l|pos l i|pos cid|pos cid|pos cid i|pos l fl|pos l fl|pos l1 l2 fl|pos cl c|pos l|pos orig res l|pos orig res|pos res|pos res|pos orig1 orig2 res|pos orig1 orig2 res|pos orig1 orig2 res|pos orig1 orig2 res|pos prem_id prem concl p]; simpl; try apply S.valid_set_clause; auto.
     - apply S.valid_set_resolve; auto.
     - apply S.valid_set_weaken; auto.
     - apply valid_check_flatten; auto; intros h1 h2 H.
@@ -420,6 +422,7 @@ Module Euf_Checker.
     - apply valid_check_distinct_elim; auto.
     - eapply valid_check_bbVar; eauto.
       apply (fun (a:Atom.atom) => BITVECTOR_LIST.zeros 0).
+    - apply valid_check_bbConst; auto.
     - apply valid_check_bbOp; auto.
     - apply valid_check_bbAdd; auto.
     - apply valid_check_bbMult; auto.
