src/lfsc/tests/bvand1.smt2
@@ -2,6 +2,7 @@
 (declare-fun a () (_ BitVec 2))
 (declare-fun b () (_ BitVec 2))
 (declare-fun c () (_ BitVec 2))
+(assert (= a #b10))
 
 (assert (= (bvand a b) c))
 (assert (not (= (bvand (bvand a b) c) c)))
